We have such list of propositions:
a) "There is velociraptor outside of my apartment";
b) "I am going to be eaten by a velociraptor";

To translate "I won't be eaten by velociraptor if there isn't a velociraptor outside my apartment" to propositional logic, it would look like: $\neg a \implies b$
Important to notice, that even our proposition has the result on the first place ("_I won't be eaten_"), we have to put it after the condition ("_if there isn't a velociraptor outside_").
So, the **only** way to write formalized proposition is to start with the condition and only then write down the result: $\neg a \implies \neg b$, not $\neg b \implies \neg a$ as it seems for the first time.
